started making the proof. realized that there's a mistake somewhere

proof.v
@@ -3,7 +3,11 @@ Require Import ZArith.
 Variable Var : Set.
 
 Variable Principal : Set.
-Definition Label := Principal -> bool.
+Variable dec_eq_Principal : forall (l1 l2:Principal), {l1=l2}+{l1<>l2}.
+Variable Label : Set.
+Variable Labels_are_functions : Label -> Principal -> bool.
+Coercion Labels_are_functions : Label >-> Funclass.
+Variable Label_ineq : forall (l1 l2:Label), l1<>l2 -> exists k, l1 k <> l2 k.
 Variable dec_eq_Label : forall (l1 l2:Label), {l1=l2}+{l1<>l2}.
 Definition flows (l1 l2 : Label) :=
   forall k, l1 k = true -> l2 k = true.
@@ -44,6 +48,7 @@ Inductive Term :=
   | TThreads : Principal -> Term -> Term -> Term
   .
 Variable subs : Term -> Var -> Term -> Term.
+Variable ffacet : PC -> Term -> Term -> Term.
 
 Inductive Context :=
   | EApp : Term -> Context
@@ -55,7 +60,18 @@ Inductive Context :=
   | ErunFacFIO : Context
   | EPut : OutputHandle -> Context
   .
-Variable fill : Context -> Term -> Term.
+Definition fill : Context -> Term -> Term :=
+  fun E t =>
+    match E with
+    | EApp t2 => TApp t t2
+    | EBindFac t2 => TBindFac t t2
+    | EPlus1 t2 => TPlus t t2
+    | EPlus2 n => TPlus (TNum n) t
+    | EIf t2 t3 => TIf t t2 t3
+    | EBindFIO t2 => TBindFIO t t2
+    | ErunFacFIO => TrunFacFIO t
+    | EPut o => TPut o t
+    end.
 
 Definition Config : Set := Term * Pointers * Inputs * Outputs.
 
@@ -110,3 +126,234 @@ Definition pO l (O:Outputs) o :=
     O o
   else
     nil.
+
+Fixpoint fac_read i p (I:Inputs) :=
+  match p with
+  | BPNum n =>
+      (TNum (list_at (I i) n), BPNum (S n))
+  | BPFacet k p1 p2 =>
+      let (t1, p1') := fac_read i p1 I  in
+      let (t2, p2') := fac_read i p2 I  in
+      (TFacet k t1 t2, BPFacet k p1' p2')
+  end.
+Definition l2pc : Label -> PC :=
+  fun l => fun k => Some (l k).
+Definition Subsumes (pc:PC) (l:Label) :=
+  forall k,
+    match pc k with
+    | Some b => b = l k
+    | None => True
+    end.
+Definition add : PC -> Principal -> PC :=
+  fun pc k1 k2 =>
+    if dec_eq_Principal k1 k2 then
+      Some true
+    else
+      pc k2.
+Definition subtract : PC -> Principal -> PC :=
+  fun pc k1 k2 =>
+    if dec_eq_Principal k1 k2 then
+      Some false
+    else
+      pc k2.
+Inductive FacStep : PC -> Config -> Config -> Prop :=
+  | FContext : forall pc t P I O t' I' O' P' E,
+      FacStep pc (t, P, I, O) (t', P', I', O') ->
+      FacStep pc (fill E t, P, I, O) (fill E t', P, I, O)
+  | FApp : forall pc x t1 t2 P I O,
+      FacStep pc (TApp (TLam x t1) t2, P, I, O) (subs t1 x t2, P, I, O)
+  | FBindFac1 : forall pc t1 t2 P I O,
+      FacStep pc (TBindFac (TRaw t1) t2, P, I, O) (TApp t2 t1, P, I, O)
+  | FBindFac2 : forall pc t1 t2 P I O,
+      FacStep pc (TBindFac (TOneFacet t1) t2, P, I, O) (TOneFacet (TBindFac t1 t2), P, I, O)
+  | FPlus : forall pc n1 n2 P I O,
+      FacStep pc (TPlus (TNum n1) (TNum n2), P, I, O) (TNum (n1+n2), P, I, O)
+  | FIf1 : forall pc t1 t2 P I O,
+      FacStep pc (TIf (TNum 0) t1 t2, P, I, O) (t1, P, I, O)
+  | FIf2 : forall pc n t1 t2 P I O,
+      n <> 0%Z ->
+      FacStep pc (TIf (TNum n) t1 t2, P, I, O) (t1, P, I, O)
+  | FBindFIO : forall pc t1 t2 P I O,
+      FacStep pc (TBindFIO (TReturn t1) t2, P, I, O) (TApp t2 t1, P, I, O)
+  | FrunFacFIO1 : forall pc t P I O,
+      FacStep pc (TrunFacFIO (TRaw t), P, I, O) (t, P, I, O)
+  | FrunFacFIO2 : forall pc t P I O,
+      FacStep pc (TrunFacFIO (TOneFacet t), P, I, O) (TrunFacFIO t, P, I, O)
+
+  | FRead : forall pc i P I O t p',
+      (t, p') = fac_read i (P i) I ->
+      FacStep pc (TGet i, P, I, O) (TReturn (ffacet (l2pc (input_label i)) t (TRaw (TNum 0))), P_upd P i p', I, O)
+  | FWrite : forall pc o n P I O,
+      Subsumes pc (output_label o) ->
+      FacStep pc (TPut o (TNum n), P, I, O) (TReturn TUnit, P, I, O_upd O o (snoc (O o) n))
+  | FWriteSkip : forall pc o n P I O,
+      not (Subsumes pc (output_label o)) ->
+      FacStep pc (TPut o (TNum n), P, I, O) (TReturn TUnit, P, I, O)
+  | FBindFac3 : forall pc k t1 t2 t3 P I O,
+      FacStep pc (TBindFac (TFacet k t1 t2) t3, P, I, O) (TFacet k (TBindFac t1 t3) (TBindFac t2 t3), P, I, O)
+  | FrunFacFIO3 : forall pc k t1 t2 P I O,
+      pc k = Some true ->
+      FacStep pc (TrunFacFIO (TFacet k t1 t2), P, I, O) (TrunFacFIO t1, P, I, O)
+  | FrunFacFIO4 : forall pc k t1 t2 P I O,
+      pc k = Some false ->
+      FacStep pc (TrunFacFIO (TFacet k t1 t2), P, I, O) (TrunFacFIO t2, P, I, O)
+  | FrunFacFIO5 : forall pc k t1 t2 P I O,
+      pc k = None ->
+      FacStep pc (TrunFacFIO (TFacet k t1 t2), P, I, O) (TThreads k (TrunFacFIO t1) (TrunFacFIO t2), P, I, O)
+  | FTimeout : forall pc E k t1 t2 P I O,
+      FacStep pc (fill E (TThreads k t1 t2), P, I, O) (TThreads k (fill E t1) (fill E t2), P, I, O)
+  | FMerge : forall pc k t1 t2 P I O,
+      FacStep pc (TThreads k (TReturn t1) (TReturn t2), P, I, O) (TReturn (TFacet k t1 t2), P, I, O)
+  | FThread1 : forall pc k t1 t2 P I O t1' P' I' O',
+      FacStep (add pc k) (t1, P, I, O) (t1', P', I', O') ->
+      FacStep pc (TThreads k t1 t2, P, I, O) (TThreads k t1' t2, P', I', O')
+  | FThread2 : forall pc k t1 t2 P I O t2' P' I' O',
+      FacStep (subtract pc k) (t2, P, I, O) (t2', P', I', O') ->
+      FacStep pc (TThreads k t1 t2, P, I, O) (TThreads k t1 t2', P', I', O')
+  .
+
+Fixpoint pt l t :=
+  match t with
+  | TFacet k t1 t2 =>
+      if l k then
+        TOneFacet (pt l t1)
+      else
+        TOneFacet (pt l t2)
+  | TThreads k t1 t2 =>
+      if l k then
+        (pt l t1)
+      else
+        (pt l t2)
+  | TPut o t =>
+      if dec_eq_Label (output_label o) l then
+        TPut o (pt l t)
+      else
+        TReturn TUnit
+  | TLam x t => TLam x (pt l t)
+  | TRaw t => TRaw (pt l t)
+  | TOneFacet t => TOneFacet (pt l t)
+  | TNum n => TNum n
+  | TUnit => TUnit
+  | TReturn t => TReturn (pt l t)
+  | TVar x => TVar x
+  | TApp t1 t2 => TApp (pt l t1) (pt l t2)
+  | TBindFac t1 t2 => TBindFac (pt l t1) (pt l t2)
+  | TPlus t1 t2 => TPlus (pt l t1) (pt l t2)
+  | TIf t1 t2 t3 => TIf (pt l t1) (pt l t2) (pt l t3)
+  | TBindFIO t1 t2 => TBindFIO (pt l t1) (pt l t2)
+  | TrunFacFIO t => TrunFacFIO (pt l t)
+  | TGet i => TGet i
+  end.
+Variable subs_lemma : forall l t1 t2 x,
+  pt l (subs t1 x t2) = subs (pt l t1) x (pt l t2).
+
+Lemma fill_lemma : forall l E t,
+  match E with
+  | EPut _ => False
+  | E => True
+  end ->
+  {E' | (pt l (fill E t)) = fill E' (pt l t)}.
+ destruct E; intros.
+        exists (EApp (pt l t)); auto.
+       exists (EBindFac (pt l t)); auto.
+      exists (EPlus1 (pt l t)); auto.
+     exists (EPlus2 z); auto.
+    exists (EIf (pt l t) (pt l t0)); auto.
+   exists (EBindFIO (pt l t)); auto.
+  exists ErunFacFIO; auto.
+ inversion H.
+Qed.
+
+Fixpoint pp (l:Label) p :=
+  match p with
+  | BPNum n => BPNum n
+  | BPFacet k p1 p2 =>
+      if l k then
+        pp l p1
+      else
+        pp l p2
+  end.
+Definition pP l (P:Pointers) i := pp l (P i).
+Definition pC (l:Label) (C:Config) : Config :=
+  match C with
+  | (t, P, I1, O1) => (pt l t, pP l P, pI l I1, pO l O1)
+  end.
+
+Definition emptypc : PC :=
+  fun k => None.
+
+Definition hints_F := (FContext, FApp, FBindFac1, FBindFac2, FPlus, FIf1, FIf2, FBindFIO, FrunFacFIO1, FrunFacFIO2, FRead, FWrite, FWriteSkip, FBindFac3, FrunFacFIO3, FrunFacFIO4, FrunFacFIO5, FTimeout, FMerge, FThread1, FThread2).
+Definition hints_S := (SContext, SApp, SBindFac1, SBindFac2, SPlus, SIf1, SIf2, SBindFIO, SrunFacFIO1, SrunFacFIO2, SRead, SWrite).
+Definition hints := (hints_F, hints_S, fill_lemma, subs_lemma).
+(*
+StdStep
+  TApp (TLam x (pt l t1)) (pt l t2)
+  pt l (subs t1 x t2)
+  (subs (pt l t1) x (pt l t2))
+*)
+
+Ltac helper := unfold pt; simpl; fold pt.
+Variable ffacet_Axiom1 : forall l1 l2 t1 t2,
+  flows l2 l1 ->
+  (pt l1 (ffacet (l2pc l2) t1 t2)) = pt l1 t1.
+Variable ffacet_Axiom2 : forall l1 l2 t1 t2,
+  not (flows l2 l1) ->
+  (pt l1 (ffacet (l2pc l2) t1 t2)) = pt l1 t2.
+
+Theorem projection_1 : forall C C' l pc,
+  FacStep pc C C' ->
+  or (pC l C = pC l C') (StdStep (pC l C) (pC l C')).
+ induction 1; unfold pC; simpl;
+(*   try solve [helper; pose (hints := hints); intuition]; *)
+ idtac.
+                     admit.
+                    helper.
+                    rewrite subs_lemma.
+                    pose (hints := hints); intuition.
+                   admit.
+                  admit.
+                 admit.
+                admit.
+               admit.
+              admit.
+             admit.
+            admit.
+           helper.
+           destruct (dec_flows (input_label i) l).
+            rewrite ffacet_Axiom1; try assumption.
+            right.
+            eapply SRead.
+
+   (* FContext *)
+   admit.
+(*
+   destruct IHFacStep.
+    left.
+    unfold pC.
+    unfold pC in H0.
+    injection H0; intros.
+    unfold fill.
+    destruct E; simpl; try congruence.
+    destruct (dec_eq_Label (output_label o) l); congruence.
+   right.
+   remember E as E_temp.
+   destruct E.
+   destruct (fill_lemma l E_temp t) as (E', H1).
+    destruct E_temp; try trivial; discriminate.
+   destruct (fill_lemma l E_temp t') as (E'', H2).
+    destruct E_temp; try trivial; discriminate.
+   unfold pC.
+   rewrite H1.
+   rewrite H2.
+   apply SContext.
+   ; try (
+    destruct (fill_lemma l E t) as (E', H1); [trivial | intuition]
+   ).
+   injection H0; intros.
+   trivial.
+   right.
+   apply SContext.
+   unfold pC.
+   rewrite fill_lemma with (t' := t').
+    trivial.
+*)
